Chase_Lev.thy
@@ -136,7 +136,7 @@ lemma chain_rewrite:
   using chain_mono unfolding pred_defs by blast
 
 definition str where
-  "str R P \<equiv> if stabilize R P = P then P else True\<^sub>p"
+  "str R P \<equiv> if P \<turnstile>\<^sub>p stabilize R P then P else True\<^sub>p"
 
 lemma str_mono:
   "Q \<turnstile>\<^sub>p P \<Longrightarrow> Q \<turnstile>\<^sub>p str R P"
@@ -146,9 +146,6 @@ subsection \<open>Trivial Cases\<close>
 
 named_theorems trivial_thms
 declare subset_UNIV [trivial_thms]
-
-lemma [trivial_thms]: "stabilize R True\<^sub>p = True\<^sub>p"
-  unfolding stabilize_def by simp
 
 lemma [trivial_thms]: "wpre a True\<^sub>p = True\<^sub>p"
   by (cases a) (auto simp:)
@@ -178,10 +175,6 @@ method pre_tac =
   (match conclusion in "Q \<subseteq> pre \<alpha> (str R P)" for \<alpha> S Q R P \<Rightarrow> \<open>succeed\<close>, pre_str_tac) |
   (match conclusion in "Q \<subseteq> pre \<alpha> P" for Q \<alpha> S P \<Rightarrow> \<open>succeed\<close>, pre_expand)
 
-method str_tac = 
-  (match conclusion in "Q \<turnstile>\<^sub>p stabilize R True\<^sub>p" for Q R \<Rightarrow> \<open>succeed\<close>, rule stabilize_univ) |
-  (match conclusion in "Q \<turnstile>\<^sub>p stabilize R (str R P)" for Q R P \<Rightarrow> \<open>succeed\<close>, rule stabilize_str) |
-  (rule stabilize_trivial, solves \<open>stabilize_trivial_tac\<close>) 
 
 
 (*
@@ -210,28 +203,116 @@ declare wpre.simps [simp del]
 method breakdown = 
   (simp add: wp_def break; intro conjI)
 
-method pre_expand = 
-  ((simp add: pre_defs guar_def
-        del: Orderings.order_top_class.top.extremum
-      split: iden.splits if_splits splits prod.splits)?; (rule subset_refl)?)
+named_theorems ops
+declare wpre.simps [ops]
+declare addI_def [ops]
+declare addR_def [ops]
+declare subR_def [ops]
+declare modR_def [ops]
+declare LE_def [ops]
 
-method pre_str_tac =
-  (rule pre_str, solves \<open>pre_expand\<close>) | 
-  (rule pre_str_mod, pre_expand)
+subsection \<open>Store Tactics\<close>
 
-method pre_tac =
-  (match conclusion in "Q \<subseteq> pre \<alpha> S UNIV" for \<alpha> S Q \<Rightarrow> \<open>succeed\<close>, rule pre_univ) |
-  (match conclusion in "Q \<subseteq> pre \<alpha> S (str R P)" for \<alpha> S Q R P \<Rightarrow> \<open>succeed\<close>, pre_str_tac) |
-  (match conclusion in "Q \<subseteq> pre \<alpha> S P" for Q \<alpha> S P \<Rightarrow> \<open>succeed\<close>, pre_expand)
+lemma sr_nop:
+  "\<forall>m. v m \<longrightarrow> P (m (ev (rg m) x :=\<^sub>s rg m e, aux: a)) = P m \<Longrightarrow> str R P \<turnstile>\<^sub>p wpre (sr v x e a) (str R P)"
+  unfolding ops pred_defs by (auto simp: str_def)
 
-method solver =
-  (match conclusion in "Q \<turnstile>\<^sub>p chain [] P" for Q P \<Rightarrow> \<open>rule chain0, (rule str_mono)?, (simp only: trivial_thms)?\<close>) |
-  (match conclusion in "Q \<turnstile>\<^sub>p chain xs P" for Q xs P \<Rightarrow> 
-    \<open>rule chain1_full, solves \<open>str_tac\<close>, solves \<open>pre_tac\<close>, solver\<close>) 
+lemma f_eq:
+  "\<forall>a. f a = g a \<Longrightarrow> f = g"
+  by auto
+
+lemma [simp]:
+  "rg (set_glb m g) = rg m"
+  by (auto simp: set_glb_def)
+
+lemma [simp]:
+  "glb (set_glb (m :: ('a, 'b, 'c) tstate_rec_scheme) (g :: ('a, 'c) gstate_rec_scheme)) = g"
+  by (auto simp: glb_def set_glb_def)
+
+lemma sr_stabilize:
+  assumes "\<And>m m'. v m' \<Longrightarrow>  R (glb m,glb m') \<Longrightarrow> ( R (glb (m(ev (rg m) x :=\<^sub>s rg m e, aux: a)),glb (m'(ev (rg m) x :=\<^sub>s rg m e, aux: a))))"
+  assumes "P \<turnstile>\<^sub>p stabilize R P" 
+  shows "wpre (sr True\<^sub>p x e a) P \<turnstile>\<^sub>p stabilize R (wpre (sr v x e a) P)"
+proof (clarsimp simp: stabilize_def pred_defs, goal_cases)
+  case (1 m g)
+  hence a: "P (m (ev (rg m) x :=\<^sub>s rg m e, aux: a))" by (auto simp: ops)
+  have b: "\<And>m m'. P m \<Longrightarrow> R (glb m,m') \<Longrightarrow> P (set_glb m m')" using assms(2) by (auto simp: stabilize_def pred_defs)
+  have r: "v (set_glb m g) \<Longrightarrow> R (glb (m(ev (rg m) x :=\<^sub>s rg m e, aux: a)), glb ((set_glb m g)(ev (rg m) x :=\<^sub>s rg m e, aux: a)))"
+    apply (rule assms(1))
+    using 1
+    by auto
+  have p: "v (set_glb m g) \<Longrightarrow> P ((set_glb m g)(ev (rg (set_glb m g)) x :=\<^sub>s rg m e, aux: a))"
+    using b[OF a,of "glb ((set_glb m g)(ev (rg m) x :=\<^sub>s rg m e, aux: a))"] r 
+    by (auto simp: set_glb_def glb_def st_upd_def aux_upd_def)
+  thus ?case by (auto simp: ops)
+qed  
+
+lemma sr_non_control:
+  assumes "\<And>m m'. v m' \<Longrightarrow>  R (glb m,glb m') \<Longrightarrow> (v m \<and> R (glb (m(ev (rg m) x :=\<^sub>s rg m e, aux: a)),glb (m'(ev (rg m) x :=\<^sub>s rg m e, aux: a))))"
+  shows "str R (wpre (sr True\<^sub>p x e a) P) \<turnstile>\<^sub>p wpre (sr v x e a) (str R P)"
+proof -
+  have "P \<turnstile>\<^sub>p stabilize R P \<Longrightarrow> wpre (sr True\<^sub>p x e a) P \<turnstile>\<^sub>p stabilize R (wpre (sr v x e a) P)"
+    apply (rule sr_stabilize)
+    using assms by auto
+  hence "P \<turnstile>\<^sub>p stabilize R P \<Longrightarrow> wpre (sr True\<^sub>p x e a) P \<turnstile>\<^sub>p stabilize R (wpre (sr True\<^sub>p x e a) P)"
+    by (auto simp: pred_defs stabilize_def ops)
+
+  thus ?thesis unfolding pred_defs str_def apply auto by (auto simp: ops)
+qed
+
+lemma sr_worse:
+  "wpre (sr v x e a) Q \<turnstile>\<^sub>p wpre (sr v x e a) (str R Q)"
+  unfolding str_def ops pred_defs by auto
+
+method sr_tac =
+  (match conclusion in "Q \<turnstile>\<^sub>p wpre (sr v x e a) (str R P)" for Q v x e a P R \<Rightarrow> \<open>succeed\<close>, 
+    solves \<open>rule sr_nop, clarsimp\<close>)
+
+subsection \<open>Load Tactics\<close>
+
+lemma ld_nop_str:
+  "\<forall>m. P (m (e :=\<^sub>r st m (ev (rg m) x), aux: a)) = P m \<Longrightarrow> str R P \<turnstile>\<^sub>p wpre (ld v x e a) (str R P)"
+  unfolding ops pred_defs by (auto simp: str_def)
+
+lemma ld_stable: (* Can we avoid introducing v again? *)
+  "v \<turnstile>\<^sub>p (\<lambda>m. \<forall>m'. R (glb m,m') \<longrightarrow> st m (ev (rg m) x) = st m' (ev (rg m) x)) \<Longrightarrow>
+    str R (wpre (ld v x e tstate_rec.more) Q) \<turnstile>\<^sub>p wpre (ld v x e tstate_rec.more) (str R Q)"
+  sorry
+
+lemma ld_worse:
+  "wpre (ld v x e tstate_rec.more) Q \<turnstile>\<^sub>p wpre (ld v x e tstate_rec.more) (str R Q)"
+  unfolding str_def ops pred_defs by auto
+
+method ld_tac =
+  (match conclusion in "Q \<turnstile>\<^sub>p wpre (ld v x e tstate_rec.more) (str R P)" for Q v x e P R \<Rightarrow> \<open>succeed\<close>, 
+    solves \<open>rule ld_nop_str, clarsimp\<close> | solves \<open>rule ld_stable, clarsimp simp: pred_defs\<close> | rule ld_worse) |    
+  (match conclusion in "Q \<turnstile>\<^sub>p wpre (sr v x e a) P" for Q v x e a P \<Rightarrow> \<open>succeed\<close>, 
+    solves \<open>rule ld_nop_str, clarsimp\<close> | blast)
+
+subsection \<open>Environment Tactics\<close>
+
+lemma env_str:
+  "str R Q \<turnstile>\<^sub>p wpre (env R) (str R Q)"
+  unfolding wpre.simps str_def by auto
+
+lemma env_fix:
+  "\<forall>m m'. Q m \<longrightarrow> R (glb m, glb m') \<longrightarrow> rg m' = rg m \<longrightarrow> Q m' \<Longrightarrow> str R Q \<turnstile>\<^sub>p wpre (env R) (Q)"
+  unfolding wpre.simps str_def by (auto simp: stabilize_def pred_defs)
+
+lemma env_worse:
+  "str R (stabilize R Q) \<turnstile>\<^sub>p wpre (env R) Q"
+  by (auto simp: str_def wpre.simps pred_defs )
+
+method env_tac =
+  (match conclusion in "Q \<turnstile>\<^sub>p wpre (env R) (str R P)" for Q R P \<Rightarrow> \<open>succeed\<close>, rule env_str) |
+  (match conclusion in "Q \<turnstile>\<^sub>p wpre (env R) P" for Q R P \<Rightarrow> \<open>succeed\<close>, rule env_fix, clarsimp)
+
+subsection \<open>Local Operation Tactics\<close>
 
 lemma ir_str:
   "str R (wpre (ir r e) Q) \<turnstile>\<^sub>p wpre (ir r e) (str R Q)"
   unfolding str_def pred_defs
+  sorry (*
 proof (clarsimp simp: wpre.simps)
   fix m assume b: "stabilize R Q = Q" "stabilize R (\<lambda>m. Q (m(r :=\<^sub>r ev (rg m) e))) \<noteq>
          (\<lambda>m. Q (m(r :=\<^sub>r ev (rg m) e)))"
@@ -246,11 +327,12 @@ proof (clarsimp simp: wpre.simps)
     unfolding stabilize_def
     by (auto simp: set_glb_def rg_upd_def)
   thus "Q (m(r :=\<^sub>r ev (rg m) e))" using b by simp
-qed
+qed *)
 
 lemma cm_str:
   "str R (wpre (cm b) Q) \<turnstile>\<^sub>p wpre (cm b) (str R Q)"
   unfolding str_def pred_defs
+  sorry (*
 proof (clarsimp simp: wpre.simps)
   fix m assume b: "stabilize R Q = Q" "stabilize R (\<lambda>m. ev\<^sub>B (rg m) b \<longrightarrow> Q m) \<noteq>
          (\<lambda>m. ev\<^sub>B (rg m) b \<longrightarrow> Q m)"
@@ -262,25 +344,108 @@ proof (clarsimp simp: wpre.simps)
     unfolding stabilize_def apply (auto simp: set_glb_def glb_def) 
     by meson
   thus "Q m" using b(2) by auto
-qed
+qed *)
 
-lemma st_str:
-  "\<forall>m m'. wpre (sr v x e a) Q m \<longrightarrow> R (glb m, glb m') \<longrightarrow> rg m' = rg m \<longrightarrow> wpre (sr v x e a) Q m' \<Longrightarrow>
-    str R (wpre (sr v x e a) Q) \<turnstile>\<^sub>p wpre (sr v x e a) (str R Q)"
+lemma ncm_str:
+  "str R (wpre (ncm b) Q) \<turnstile>\<^sub>p wpre (cm b) (str R Q)"
   unfolding str_def pred_defs
   sorry
 
-lemma ld_str:
-  "\<forall>m m'. wpre (ld v x e a) Q m \<longrightarrow> R (glb m, glb m') \<longrightarrow> rg m' = rg m \<longrightarrow> wpre (ld v x e a) Q m' \<Longrightarrow>
-    str R (wpre (ld v x e a) Q) \<turnstile>\<^sub>p wpre (ld v x e a) (str R Q)"
-  unfolding str_def pred_defs
+method local_tac =
+  (match conclusion in "Q \<turnstile>\<^sub>p wpre (ir r e) (str R P)" for Q e r R P \<Rightarrow> \<open>succeed\<close>, rule ir_str) |
+  (match conclusion in "Q \<turnstile>\<^sub>p wpre (cm b) (str R P)" for Q b R P \<Rightarrow> \<open>succeed\<close>, rule cm_str) |
+  (match conclusion in "Q \<turnstile>\<^sub>p wpre (ncm b) (str R P)" for Q b R P \<Rightarrow> \<open>succeed\<close>, rule ncm_str)
+
+
+subsection \<open>General Tactics\<close>
+
+lemma [simp]:
+  "rg (m(a :=\<^sub>r e)) b = (if a = b then e else rg m b)"
+  by (auto simp: rg_upd_def)
+
+lemma [simp]:
+  "st (m(a :=\<^sub>r e)) b = st m b"
+  by (auto simp: rg_upd_def)
+
+lemma [simp]:
+  "st (m(a :=\<^sub>s e)) b = (if a = b then e else st m b)"
+  by (auto simp: st_upd_def)
+
+lemma [simp]:
+  "tstate_rec.more (m(a :=\<^sub>s e)) = tstate_rec.more m"
+  by (auto simp: st_upd_def)
+
+lemma [simp]:
+  "gstate_rec.more (m(a :=\<^sub>s e)) = gstate_rec.more m"
+  by (auto simp: st_upd_def)
+
+lemma [simp]:
+  "rg (m(a :=\<^sub>s e)) b = rg m b"
+  by (auto simp: st_upd_def)
+
+lemma [simp]:
+  "st (glb m) x = st m x"
+  by (auto simp: glb_def)
+
+lemma [simp]:
+  "gstate_rec.more (glb m) x = tstate_rec.more m x"
+  by (auto simp: glb_def)
+
+lemma [simp]:
+  "tstate_rec.more (set_glb m g) = gstate_rec.more g"
+  by (auto simp: set_glb_def)
+
+lemma [simp]:
+  "(set_glb m g)(r :=\<^sub>r e) = set_glb (m(r :=\<^sub>r e)) g"
+  by (auto simp: set_glb_def rg_upd_def)
+
+lemma [simp]:
+  "(set_glb m g)(r :=\<^sub>s e) = set_glb m (g(r :=\<^sub>s e))"
+  by (auto simp: set_glb_def st_upd_def)
+
+lemma [simp]:
+  "glb (m(r :=\<^sub>s e)) = (glb m)(r :=\<^sub>s e)"
+  by (auto simp: glb_def st_upd_def)
+
+method solver =
+  (match conclusion in "Q \<turnstile>\<^sub>p True\<^sub>p" for Q \<Rightarrow> \<open>simp add: pred_defs\<close>) |
+  (match conclusion in "Q \<turnstile>\<^sub>p chain x True\<^sub>p" for x Q \<Rightarrow> \<open>simp add: trivial_thms pred_defs\<close>) |
+  (match conclusion in "Q \<turnstile>\<^sub>p chain [] P" for Q P \<Rightarrow> 
+    \<open>rule chain0, (rule str_mono)?, (simp only: trivial_thms)?, auto simp: pred_defs\<close>) |
+  (match conclusion in "Q \<turnstile>\<^sub>p chain (sr v x e a#xs) P" for Q v x e a xs P \<Rightarrow> 
+    \<open>rule chain1_full, solves \<open>sr_tac\<close>, (simp add: ops)?\<close>) | 
+  (match conclusion in "Q \<turnstile>\<^sub>p chain (ld v x e a#xs) P" for Q v x e a xs P \<Rightarrow> 
+    \<open>rule chain1_full, solves \<open>ld_tac\<close>, (simp add: ops)?\<close>) | 
+  (match conclusion in "Q \<turnstile>\<^sub>p chain (env R#xs) P" for Q R xs P \<Rightarrow> 
+    \<open>rule chain1_full, solves \<open>env_tac\<close>\<close>) |
+  (match conclusion in "Q \<turnstile>\<^sub>p chain (ir r e#xs) P" for Q r e xs P \<Rightarrow> 
+    \<open>rule chain1_full, solves \<open>local_tac\<close>, simp add: ops\<close>)  |
+  (match conclusion in "Q \<turnstile>\<^sub>p chain (cm b#xs) P" for Q b xs P \<Rightarrow> 
+    \<open>rule chain1_full, solves \<open>local_tac\<close>, simp add: ops\<close>) |
+  (match conclusion in "Q \<turnstile>\<^sub>p chain (ncm b#xs) P" for Q b xs P \<Rightarrow> 
+    \<open>rule chain1_full, solves \<open>local_tac\<close>, simp add: ops\<close>) 
+
+
+
+lemma chain0_str:
+  "P \<turnstile>\<^sub>p Q \<Longrightarrow> P \<turnstile>\<^sub>p  chain [] (str R Q)"
+  unfolding chain.simps str_def pred_defs by auto
+
+lemma [simp]:
+  "str R True\<^sub>p = True\<^sub>p"
+  by (auto simp: str_def)
+
+lemma rewrite_tac:
+  "P \<turnstile>\<^sub>p Q \<Longrightarrow> X \<turnstile>\<^sub>p chain x P \<Longrightarrow> X \<turnstile>\<^sub>p chain x Q"
   sorry
 
-
-lemma env_str:
-  "str R Q \<turnstile>\<^sub>p wpre (env R) (str R Q)"
+lemma str_tac:
+  "P \<turnstile>\<^sub>p stabilize R P \<Longrightarrow> str R P \<turnstile>\<^sub>p P"
   sorry
 
+lemma env_fix':
+  "Q \<turnstile>\<^sub>p stabilize R Q \<Longrightarrow> str R Q \<turnstile>\<^sub>p wpre (env R) (Q)"
+  unfolding wpre.simps str_def by (auto simp: stabilize_def pred_defs)
 
 lemma chase_lev_put:
    "TOP = PTR \<Longrightarrow> BOT = PTR + 1 \<Longrightarrow> LEN = PTR + 2 \<Longrightarrow> BUF = PTR + 3 \<Longrightarrow> 
@@ -289,7 +454,7 @@ lemma chase_lev_put:
       R: =[BOT] \<and> \<le>[TOP] \<and> =[BUF] \<and> =[LEN] \<and> =[(BUF + (\<^sup>1[BOT] mod \<^sup>1[LEN]))] \<and> (\<^sup>1\<^sup>adeque,\<^sup>2\<^sup>adeque) \<in> S\<^sup>*
       G: \<le>[BOT] \<and> =[TOP] \<and> =[LEN]
       I: \<^sup>adeque = \<acute>(queue PTR) \<and> \<^sup>s[TOP] \<le> \<^sup>s[BOT]
-      P: \<^sup>rr\<^sub>0 = PTR \<and> V = \<^sup>rr\<^sub>1 \<and> A = \<^sup>adeque \<and> SPACE = (\<^sup>s[BOT] - \<^sup>s[TOP] < \<^sup>s[LEN])
+      P: \<^sup>rr\<^sub>0 = PTR \<and> V = \<^sup>rr\<^sub>1 \<and> D = \<^sup>adeque \<and> SPACE = (\<^sup>s[BOT] - \<^sup>s[TOP] < \<^sup>s[LEN])
       {
         \<lbrace> \<^sup>rr\<^sub>0 = PTR \<rbrace> r\<^sub>2 := [r\<^sub>0 + #0];
         \<lbrace> \<^sup>rr\<^sub>0 = PTR \<rbrace> r\<^sub>3 := [r\<^sub>0 + #1];
@@ -299,25 +464,136 @@ lemma chase_lev_put:
           r\<^sub>2 := r\<^sub>3 % r\<^sub>4;
           r\<^sub>2 := r\<^sub>2 + r\<^sub>0;
           r\<^sub>2 := r\<^sub>2 + #3;
-          \<lbrace> \<^sup>rr\<^sub>2 = BUF + (\<^sup>s[BOT] mod \<^sup>s[LEN]) \<and> \<^sup>s[BOT] - \<^sup>s[TOP] < \<^sup>s[LEN] \<rbrace> 
+          \<lbrace> \<^sup>rr\<^sub>2 = BUF + (\<^sup>s[BOT] mod \<^sup>s[LEN]) \<and> (\<forall>i. \<^sup>s[TOP] \<le> i \<longrightarrow> \<^sup>s[BOT] - i < \<^sup>s[LEN]) \<rbrace> 
             [r\<^sub>2 + #0] := r\<^sub>1;
           fence;
           r\<^sub>3 := r\<^sub>3 + #1;
-          \<lbrace> \<^sup>rr\<^sub>0 = PTR \<and> \<^sup>rr\<^sub>3 = \<^sup>s[BOT]+1 \<and> \<^sup>rr\<^sub>1 = \<^sup>s[BUF + (\<^sup>s[BOT] mod \<^sup>s[LEN])] \<and> \<^sup>s[BOT] - \<^sup>s[TOP] < \<^sup>s[LEN] \<rbrace> 
+          \<lbrace> \<^sup>rr\<^sub>0 = PTR \<and> \<^sup>rr\<^sub>3 = \<^sup>s[BOT]+1 \<and> \<^sup>rr\<^sub>1 = \<^sup>s[BUF + (\<^sup>s[BOT] mod \<^sup>s[LEN])] \<and> (\<forall>i. \<^sup>s[TOP] \<le> i \<longrightarrow> \<^sup>s[BOT] - i < \<^sup>s[LEN]) \<rbrace> 
             [r\<^sub>0 + #1] := r\<^sub>3, \<^sup>adeque := \<^sup>adeque@[\<^sup>rr\<^sub>1]
         fi
       }
-      Q: SPACE \<longrightarrow> (A,\<^sup>adeque) \<in> S\<^sup>* O (put V) O S\<^sup>*
+      Q: SPACE \<longrightarrow> (D,\<^sup>adeque) \<in> S\<^sup>* O (put V) O S\<^sup>*
     FNEND" 
   apply (clarsimp simp add: local_props_def, intro conjI)
   prefer 10
-
   apply (simp add: break, intro conjI; simp only: append.simps chain_singleI' chain_singleI chain_lastI)
 
   apply (rule chain1_full)
-  apply (blast)
-  apply (simp add: wpre.simps)
-  apply (simp add: break, intro conjI)
+  apply blast
+  apply (clarsimp simp: ops st_upd_def aux_upd_def)
+
+  apply (rule chain1_full)
+  apply (rule env_fix')
+  apply (auto simp: pred_defs stabilize_def)[1]
+  apply (smt glb_def gstate_rec.ext_inject gstate_rec.surjective relcomp.relcompI rtrancl_trans)
+
+  apply solver+n
+
+  sorry
+
+  apply (rule chain1_full)
+  apply (rule env_worse)
+  apply (auto simp: stabilize_def)[1]
+  apply solver
+  apply (auto simp: pred_defs)[1]
+
+  apply solver+
+
+  apply (rule chain1_full)
+  apply (rule sr_worse)
+  apply (clarsimp simp: ops)
+  apply solver+
+
+  apply (rule chain1_full)
+  apply (rule env_worse)
+  apply (auto simp: stabilize_def)[1]
+  apply solver
+  apply (auto simp: pred_defs)[1]
+
+  apply (rule chain1_full)
+  apply blast
+  apply (clarsimp simp: ops aux_upd_def st_upd_def o_def)
+
+  apply (rule chain1_full)
+  apply (rule env_worse)
+  apply (auto simp: stabilize_def)[1]
+
+  apply solver+
+
+  apply (rule chain1_full)
+  apply (rule sr_worse)
+  apply (clarsimp simp: ops)
+
+  apply (rule chain1_full)
+  apply (rule env_worse)
+  apply (auto simp: stabilize_def)[1]
+
+  apply solver+
+
+apply (rule chain1_full)
+  apply (rule env_worse)
+  apply (auto simp: stabilize_def)[1]
+
+  apply solver
+
+  unfolding pred_defs
+
+  apply clarsimp
+  apply (intro conjI impI allI)
+  apply simp
+
+  apply (auto simp: st_upd_def glb_def rg_upd_def set_glb_def)[1]
+  unfolding put_def 
+  defer 1
+  defer 1
+
+  apply solver
+
+  sorry
+
+  apply solver
+  apply solver
+
+
+  apply solver
+  apply solver
+  apply solver
+  apply solver
+  apply solver
+
+  apply (rule chain1_full)
+  apply (rule ld_stable)
+  apply (clarsimp simp: pred_defs glb_def)
+
+  apply solver
+  apply solver
+
+  apply (rule chain1_full)
+  apply (rule ld_stable)
+  apply (clarsimp simp: pred_defs glb_def)
+  apply (clarsimp simp: ops)
+
+  apply solver
+
+  apply (rule rewrite_str[of "\<lambda>m. rg m r\<^sub>0 = PTR"])
+  apply (clarsimp simp: pred_defs glb_def)
+
+  apply (rule chain1_full)
+  apply (rule ld_worse)
+  apply (clarsimp simp: ops)
+
+  apply (rule chain1_full)
+  apply (rule env_worse)
+  apply (clarsimp simp: stabilize_def)
+
+
+
+  sorry
+
+  apply (rule chain1_full)
+  apply (solves \<open>env_tac\<close>)
+  apply auto[1]
+
   sorry
 
   apply (rule chain1_full)
